theories/Monad.v
@@ -1,0 +1,125 @@
+From LogRel.AutoSubst Require Import core unscoped Ast Extra.
+Require Import PeanoNat.
+From LogRel Require Import Utils BasicAst Notations Context LContexts NormalForms Weakening GenericTyping.
+
+Record Psh (wl : wfLCon) :=
+  { typ : forall wl',  wl' ≤ε wl -> Type ;
+    mon : forall wl' wl''  (alpha : wl' ≤ε wl) (beta : wl'' ≤ε wl')
+    (delta : wl'' ≤ε wl),
+      typ wl' alpha -> typ wl'' delta
+  }.
+
+Arguments typ [_] _.
+Arguments mon [_ _ _] _.
+
+Record Weak (wl : wfLCon) (P : forall wl', wl' ≤ε wl  -> Type) : Type :=
+  { PN : nat ;
+    WP : forall (wl' : wfLCon) (alpha : wl' ≤ε wl),
+      AllInLCon PN wl' -> P wl' alpha ;
+  }.
+
+
+Lemma monot (wl wl' wl'' : wfLCon)
+  (P : forall wl',  wl' ≤ε wl -> Type)
+  (alpha :  wl' ≤ε wl)
+  (beta :  wl'' ≤ε wl') :
+  Weak wl' (fun wl'' dzeta => P wl'' (dzeta •ε alpha)) ->
+  Weak wl'' (fun wl''' dzeta => P wl''' ((dzeta •ε beta) •ε alpha)).
+Proof.
+  intros [N WN].
+  exists N.
+  intros wl''' dzeta allinl.
+  exact (WN wl''' (dzeta •ε beta) allinl).
+Qed.  
+
+
+Definition Wbind (wl : wfLCon) (P Q : forall wl', wl' ≤ε wl  -> Type)
+  (Pe : forall wl' (alpha : wl' ≤ε wl) wl'' (beta : wl'' ≤ε wl),
+      wl'' ≤ε wl' -> P wl' alpha -> P wl'' beta)
+  (Qe : forall wl' (alpha : wl' ≤ε wl) wl'' (beta : wl'' ≤ε wl),
+      wl'' ≤ε wl' -> Q wl' alpha -> Q wl'' beta)
+  (f : forall wl' (alpha : wl' ≤ε wl),
+      P wl' alpha -> Weak wl' (fun wl'' beta => Q wl'' (beta •ε alpha))) :
+  forall wl' (alpha : wl' ≤ε wl),
+    Weak wl' (fun wl'' beta => P wl'' (beta •ε alpha)) ->
+    Weak wl' (fun wl'' beta => Q wl'' (beta •ε alpha)).
+Proof.
+  intros * [N W].
+  unshelve econstructor.
+  { unshelve eapply (max N _).
+    unshelve eapply Max_Bar.
+    - exact wl'.
+    - exact N.
+    - intros wl'' beta allinl.
+      unshelve eapply (f wl'' (beta •ε alpha)).
+      now eapply W.
+  }
+  intros wl'' beta allinl.
+  unshelve eapply Qe.
+  4: unshelve eapply f.
+  { unshelve eapply (Bar_lub (Bar_lub wl' wl'' N beta _) wl'').
+    3: now eapply Bar_lub_smaller.
+    3: eassumption.
+    eapply AllInLCon_le.
+    eapply Nat.le_max_l.
+    eassumption.
+  }
+  + unshelve eapply Bar_lub_smaller.
+  + eapply (Bar_lub wl' wl'' N beta _).
+  + now eapply Bar_lub_ub.
+  + unshelve eapply (_ •ε alpha).
+    now eapply Bar_lub_ub.
+  + eapply W.
+    now eapply Bar_lub_AllInLCon.
+  + eapply AllInLCon_le ; [ | now eapply Bar_lub_AllInLCon].
+    etransitivity ; [ |now eapply Nat.le_max_r].
+    etransitivity ; [ | now eapply Max_Bar_Bar_lub].
+    cbn.
+    reflexivity.
+Qed.    
+
+
+Definition Wret (wl : wfLCon) (P : forall wl', wl' ≤ε wl  -> Type)
+  (Pe : forall wl' (alpha : wl' ≤ε wl) wl'' (beta : wl'' ≤ε wl),
+      wl'' ≤ε wl' -> P wl' alpha -> P wl'' beta)
+  (p : P wl (idε wl)) : Weak wl P.
+Proof.
+  unshelve econstructor.
+  - exact 0.
+  - intros ; now eapply Pe.
+Defined.
+
+
+(*
+Definition Wbind (wl : wfLCon) (P Q : wfLCon -> Type)
+  (Pe : forall wl' wl'', wl'' ≤ε wl' -> P wl' -> P wl'')
+  (Qe : forall wl' wl'', wl'' ≤ε wl' -> Q wl' -> Q wl'')
+  (f : forall wl', wl' ≤ε wl -> P wl' -> Weak wl' Q)
+  (p : Weak wl P) : Weak wl Q.
+Proof.
+  unshelve econstructor.
+  - unshelve refine (max (PN wl P p) (Max_Bar _ _ _)).
+    + exact wl.
+    + exact (PN _ _ p).
+    + intros wl' tau Ninfl.
+      eapply PN.
+      eapply f.
+      * eassumption.
+      * eapply WP ; try eassumption.
+  - intros wl' tau Ninfl.
+    unshelve eapply WP.
+    4:{ eapply AllInLCon_le ; try eassumption.
+        etransitivity.
+        eapply (Max_Bar_Bar_lub _ _
+                  (fun wl'0 tau0 Ninfl0 => PN wl'0 Q (f wl'0 tau0 (WP wl P p wl'0 tau0 Ninfl0)))).
+        eapply Nat.le_max_r.
+    }
+    eapply Bar_lub_smaller.
+    Unshelve.
+    + eassumption.
+    + eapply AllInLCon_le ; try eassumption.
+      now eapply Nat.le_max_l.
+    + now eapply Bar_lub_ub.
+    + now eapply Bar_lub_AllInLCon.
+Defined.      
+*)
